More work in progress on executable parse_opcode

vfmOperationScript.sml
@@ -156,8 +156,8 @@ Definition opcode_def:
   ∧ opcode Gas            = [n2w 0x5a]
   ∧ opcode JumpDest       = [n2w 0x5b]
   ∧ opcode (Push n w)     = [n2w 0x5f + w2w n] ++ w
-  ∧ opcode (Dup n)        = [n2w 0x81 + w2w n]
-  ∧ opcode (Swap n)       = [n2w 0x91 + w2w n]
+  ∧ opcode (Dup n)        = [n2w 0x80 + w2w n]
+  ∧ opcode (Swap n)       = [n2w 0x90 + w2w n]
   ∧ opcode (Log n)        = [n2w 0xa0 + w2w n]
   ∧ opcode Create         = [n2w 0xf0]
   ∧ opcode Call           = [n2w 0xf1]
@@ -173,12 +173,298 @@ Definition invalid_opcode_def:
   invalid_opcode : byte = n2w 0xfe
 End
 
-open cv_transLib cv_stdTheory;
-
 Definition parse_opcode_def:
   parse_opcode (opc:byte list) =
     some opn. wf_opname opn ∧ opcode opn ≼ opc
 End
+
+Definition static_gas_def[simp]:
+    static_gas Stop           = 0
+  ∧ static_gas Add            = 3
+  ∧ static_gas Mul            = 5
+  ∧ static_gas Sub            = 3
+  ∧ static_gas Div            = 5
+  ∧ static_gas SDiv           = 5
+  ∧ static_gas Mod            = 5
+  ∧ static_gas SMod           = 5
+  ∧ static_gas AddMod         = 8
+  ∧ static_gas MulMod         = 8
+  ∧ static_gas Exp            = 10
+  ∧ static_gas SignExtend     = 5
+  ∧ static_gas LT             = 3
+  ∧ static_gas GT             = 3
+  ∧ static_gas SLT            = 3
+  ∧ static_gas SGT            = 3
+  ∧ static_gas Eq             = 3
+  ∧ static_gas IsZero         = 3
+  ∧ static_gas And            = 3
+  ∧ static_gas Or             = 3
+  ∧ static_gas XOr            = 3
+  ∧ static_gas Not            = 3
+  ∧ static_gas Byte           = 3
+  ∧ static_gas ShL            = 3
+  ∧ static_gas ShR            = 3
+  ∧ static_gas SAR            = 3
+  ∧ static_gas Keccak256      = 30
+  ∧ static_gas Address        = 30
+  ∧ static_gas Balance        = 0
+  ∧ static_gas Origin         = 2
+  ∧ static_gas Caller         = 2
+  ∧ static_gas CallValue      = 2
+  ∧ static_gas CallDataLoad   = 3
+  ∧ static_gas CallDataSize   = 2
+  ∧ static_gas CallDataCopy   = 3
+  ∧ static_gas CodeSize       = 2
+  ∧ static_gas CodeCopy       = 3
+  ∧ static_gas GasPrice       = 2
+  ∧ static_gas ExtCodeSize    = 0
+  ∧ static_gas ExtCodeCopy    = 0
+  ∧ static_gas ReturnDataSize = 2
+  ∧ static_gas ReturnDataCopy = 3
+  ∧ static_gas ExtCodeHash    = 0
+  ∧ static_gas BlockHash      = 20
+  ∧ static_gas CoinBase       = 2
+  ∧ static_gas TimeStamp      = 2
+  ∧ static_gas Number         = 2
+  ∧ static_gas PrevRandao     = 2
+  ∧ static_gas GasLimit       = 2
+  ∧ static_gas ChainId        = 2
+  ∧ static_gas SelfBalance    = 5
+  ∧ static_gas BaseFee        = 2
+  ∧ static_gas Pop            = 2
+  ∧ static_gas MLoad          = 3
+  ∧ static_gas MStore         = 3
+  ∧ static_gas MStore8        = 3
+  ∧ static_gas SLoad          = 0
+  ∧ static_gas SStore         = 0
+  ∧ static_gas Jump           = 8
+  ∧ static_gas JumpI          = 10
+  ∧ static_gas PC             = 2
+  ∧ static_gas MSize          = 2
+  ∧ static_gas Gas            = 2
+  ∧ static_gas JumpDest       = 1
+  ∧ static_gas (Push n w)     = (if n = 0w then 2 else 3)
+  ∧ static_gas (Dup n)        = 3
+  ∧ static_gas (Swap n)       = 3
+  ∧ static_gas (Log n)        = 375
+  ∧ static_gas Create         = 32000
+  ∧ static_gas Call           = 0
+  ∧ static_gas CallCode       = 0
+  ∧ static_gas Return         = 0
+  ∧ static_gas DelegateCall   = 0
+  ∧ static_gas Create2        = 32000
+  ∧ static_gas StaticCall     = 0
+  ∧ static_gas Revert         = 0
+End
+
+(*
+Theorem parse_opcode_cond_thm:
+  parse_opcode (opc::rest: byte list) =
+  if opc = n2w 0x00 then SOME Stop else
+  if opc = n2w 0x01 then SOME Add else
+  if opc = n2w 0x02 then SOME Mul else
+  if opc = n2w 0x03 then SOME Sub else
+  if opc = n2w 0x04 then SOME Div else
+  if opc = n2w 0x05 then SOME SDiv else
+  if opc = n2w 0x06 then SOME Mod else
+  if opc = n2w 0x07 then SOME SMod else
+  if opc = n2w 0x08 then SOME AddMod else
+  if opc = n2w 0x09 then SOME MulMod else
+  if opc = n2w 0x0a then SOME Exp else
+  if opc = n2w 0x0b then SOME SignExtend else
+  if opc = n2w 0x10 then SOME LT else
+  if opc = n2w 0x11 then SOME GT else
+  if opc = n2w 0x12 then SOME SLT else
+  if opc = n2w 0x13 then SOME SGT else
+  if opc = n2w 0x14 then SOME Eq else
+  if opc = n2w 0x15 then SOME IsZero else
+  if opc = n2w 0x16 then SOME And else
+  if opc = n2w 0x17 then SOME Or else
+  if opc = n2w 0x18 then SOME XOr else
+  if opc = n2w 0x19 then SOME Not else
+  if opc = n2w 0x1a then SOME Byte else
+  if opc = n2w 0x1b then SOME ShL else
+  if opc = n2w 0x1c then SOME ShR else
+  if opc = n2w 0x1d then SOME SAR else
+  if opc = n2w 0x20 then SOME Keccak256 else
+  if opc = n2w 0x30 then SOME Address else
+  if opc = n2w 0x31 then SOME Balance else
+  if opc = n2w 0x32 then SOME Origin else
+  if opc = n2w 0x33 then SOME Caller else
+  if opc = n2w 0x34 then SOME CallValue else
+  if opc = n2w 0x35 then SOME CallDataLoad else
+  if opc = n2w 0x36 then SOME CallDataSize else
+  if opc = n2w 0x37 then SOME CallDataCopy else
+  if opc = n2w 0x38 then SOME CodeSize else
+  if opc = n2w 0x39 then SOME CodeCopy else
+  if opc = n2w 0x3a then SOME GasPrice else
+  if opc = n2w 0x3b then SOME ExtCodeSize else
+  if opc = n2w 0x3c then SOME ExtCodeCopy else
+  if opc = n2w 0x3d then SOME ReturnDataSize else
+  if opc = n2w 0x3e then SOME ReturnDataCopy else
+  if opc = n2w 0x3f then SOME ExtCodeHash else
+  if opc = n2w 0x40 then SOME BlockHash else
+  if opc = n2w 0x41 then SOME CoinBase else
+  if opc = n2w 0x42 then SOME TimeStamp else
+  if opc = n2w 0x43 then SOME Number else
+  if opc = n2w 0x44 then SOME PrevRandao else
+  if opc = n2w 0x45 then SOME GasLimit else
+  if opc = n2w 0x46 then SOME ChainId else
+  if opc = n2w 0x47 then SOME SelfBalance else
+  if opc = n2w 0x48 then SOME BaseFee else
+  if opc = n2w 0x50 then SOME Pop else
+  if opc = n2w 0x51 then SOME MLoad else
+  if opc = n2w 0x52 then SOME MStore else
+  if opc = n2w 0x53 then SOME MStore8 else
+  if opc = n2w 0x54 then SOME SLoad else
+  if opc = n2w 0x55 then SOME SStore else
+  if opc = n2w 0x56 then SOME Jump else
+  if opc = n2w 0x57 then SOME JumpI else
+  if opc = n2w 0x58 then SOME PC else
+  if opc = n2w 0x59 then SOME MSize else
+  if opc = n2w 0x5a then SOME Gas else
+  if opc = n2w 0x5b then SOME JumpDest else
+  if opc = n2w 0x5f then SOME (Push 0w  (TAKE 0 rest)) else
+  if opc = n2w 0x60 then SOME (Push 1w  (TAKE 1 rest)) else
+  if opc = n2w 0x61 then SOME (Push 2w  (TAKE 2 rest)) else
+  if opc = n2w 0x62 then SOME (Push 3w  (TAKE 3 rest)) else
+  if opc = n2w 0x63 then SOME (Push 4w  (TAKE 4 rest)) else
+  if opc = n2w 0x64 then SOME (Push 5w  (TAKE 5 rest)) else
+  if opc = n2w 0x65 then SOME (Push 6w  (TAKE 6 rest)) else
+  if opc = n2w 0x66 then SOME (Push 7w  (TAKE 7 rest)) else
+  if opc = n2w 0x67 then SOME (Push 8w  (TAKE 8 rest)) else
+  if opc = n2w 0x68 then SOME (Push 9w  (TAKE 9 rest)) else
+  if opc = n2w 0x69 then SOME (Push 10w (TAKE 10 rest)) else
+  if opc = n2w 0x6a then SOME (Push 11w (TAKE 11 rest)) else
+  if opc = n2w 0x6b then SOME (Push 12w (TAKE 12 rest)) else
+  if opc = n2w 0x6c then SOME (Push 13w (TAKE 13 rest)) else
+  if opc = n2w 0x6d then SOME (Push 14w (TAKE 14 rest)) else
+  if opc = n2w 0x6e then SOME (Push 15w (TAKE 15 rest)) else
+  if opc = n2w 0x6f then SOME (Push 16w (TAKE 16 rest)) else
+  if opc = n2w 0x70 then SOME (Push 17w (TAKE 17 rest)) else
+  if opc = n2w 0x71 then SOME (Push 18w (TAKE 18 rest)) else
+  if opc = n2w 0x72 then SOME (Push 19w (TAKE 19 rest)) else
+  if opc = n2w 0x73 then SOME (Push 20w (TAKE 20 rest)) else
+  if opc = n2w 0x74 then SOME (Push 21w (TAKE 21 rest)) else
+  if opc = n2w 0x75 then SOME (Push 22w (TAKE 22 rest)) else
+  if opc = n2w 0x76 then SOME (Push 23w (TAKE 23 rest)) else
+  if opc = n2w 0x77 then SOME (Push 24w (TAKE 24 rest)) else
+  if opc = n2w 0x78 then SOME (Push 25w (TAKE 25 rest)) else
+  if opc = n2w 0x79 then SOME (Push 26w (TAKE 26 rest)) else
+  if opc = n2w 0x7a then SOME (Push 27w (TAKE 27 rest)) else
+  if opc = n2w 0x7b then SOME (Push 28w (TAKE 28 rest)) else
+  if opc = n2w 0x7c then SOME (Push 29w (TAKE 29 rest)) else
+  if opc = n2w 0x7d then SOME (Push 30w (TAKE 30 rest)) else
+  if opc = n2w 0x7e then SOME (Push 31w (TAKE 31 rest)) else
+  if opc = n2w 0x7f then SOME (Push 32w (TAKE 32 rest)) else
+  if opc = n2w 0x80 then SOME (Dup 0w) else
+  if opc = n2w 0x81 then SOME (Dup 1w) else
+  if opc = n2w 0x82 then SOME (Dup 2w) else
+  if opc = n2w 0x83 then SOME (Dup 3w) else
+  if opc = n2w 0x84 then SOME (Dup 4w) else
+  if opc = n2w 0x85 then SOME (Dup 5w) else
+  if opc = n2w 0x86 then SOME (Dup 6w) else
+  if opc = n2w 0x87 then SOME (Dup 7w) else
+  if opc = n2w 0x88 then SOME (Dup 8w) else
+  if opc = n2w 0x89 then SOME (Dup 9w) else
+  if opc = n2w 0x8a then SOME (Dup 10w) else
+  if opc = n2w 0x8b then SOME (Dup 11w) else
+  if opc = n2w 0x8c then SOME (Dup 12w) else
+  if opc = n2w 0x8d then SOME (Dup 13w) else
+  if opc = n2w 0x8e then SOME (Dup 14w) else
+  if opc = n2w 0x8f then SOME (Dup 15w) else
+  if opc = n2w 0x90 then SOME (Swap 0w) else
+  if opc = n2w 0x91 then SOME (Swap 1w) else
+  if opc = n2w 0x92 then SOME (Swap 2w) else
+  if opc = n2w 0x93 then SOME (Swap 3w) else
+  if opc = n2w 0x94 then SOME (Swap 4w) else
+  if opc = n2w 0x95 then SOME (Swap 5w) else
+  if opc = n2w 0x96 then SOME (Swap 6w) else
+  if opc = n2w 0x97 then SOME (Swap 7w) else
+  if opc = n2w 0x98 then SOME (Swap 8w) else
+  if opc = n2w 0x99 then SOME (Swap 9w) else
+  if opc = n2w 0x9a then SOME (Swap 10w) else
+  if opc = n2w 0x9b then SOME (Swap 11w) else
+  if opc = n2w 0x9c then SOME (Swap 12w) else
+  if opc = n2w 0x9d then SOME (Swap 13w) else
+  if opc = n2w 0x9e then SOME (Swap 14w) else
+  if opc = n2w 0x9f then SOME (Swap 15w) else
+  if opc = n2w 0xa0 then SOME (Log 0w) else
+  if opc = n2w 0xa1 then SOME (Log 1w) else
+  if opc = n2w 0xa2 then SOME (Log 2w) else
+  if opc = n2w 0xa3 then SOME (Log 3w) else
+  if opc = n2w 0xf0 then SOME Create else
+  if opc = n2w 0xf1 then SOME Call else
+  if opc = n2w 0xf2 then SOME CallCode else
+  if opc = n2w 0xf3 then SOME Return else
+  if opc = n2w 0xf4 then SOME DelegateCall else
+  if opc = n2w 0xf5 then SOME Create2 else
+  if opc = n2w 0xfa then SOME StaticCall else
+  if opc = n2w 0xfd then SOME Revert else
+  NONE
+Proof
+  simp[parse_opcode_def]
+  \\ DEEP_INTRO_TAC some_intro
+  \\ rw[]
+  \\ TRY (
+    rename1`Push 32w (TAKE 32 _)`
+    \\ rename1`opcode opc`
+    \\ Cases_on`opc`
+    \\ qpat_x_assum`_ ≼ _`mp_tac
+    \\ qpat_x_assum`wf_opname _`mp_tac
+    \\ simp_tac(srw_ss())[opcode_def]
+    \\ TRY(blastLib.BBLAST_TAC \\ NO_TAC)
+    \\ ntac 2 strip_tac
+    \\ conj_asm1_tac >- (
+      qpat_x_assum`_ = _`mp_tac
+      \\ blastLib.BBLAST_TAC)
+    \\ rw[] \\ fs[rich_listTheory.IS_PREFIX_APPEND]
+    \\ rw[rich_listTheory.TAKE_APPEND]
+  )
+  \\ TRY (
+    rename1`opcode opc`
+    \\ Cases_on`opc`
+    \\ qpat_x_assum`_ ≼ _`mp_tac
+    \\ qpat_x_assum`wf_opname _`mp_tac
+    \\ simp_tac(srw_ss())[opcode_def]
+    \\ blastLib.BBLAST_TAC
+    )
+QED
+
+
+  \\ tac
+  THENL (List.tabulate(until, fn _ => tac) @
+         List.tabulate(282 - until, fn _ => ALL_TAC))
+
+val until = 130
+val tac =
+    rename1`opcode opc`
+    \\ Cases_on`opc`
+    \\ qpat_x_assum`_ ≼ _`mp_tac
+    \\ qpat_x_assum`wf_opname _`mp_tac
+    \\ simp_tac(srw_ss())[opcode_def]
+    \\ blastLib.BBLAST_TAC
+
+  \\ TRY(
+    rename1`opcode opc`
+    \\ Cases_on`opc`
+    \\ qpat_x_assum`_ ≼ _`mp_tac
+    \\ qpat_x_assum`wf_opname _`mp_tac
+    \\ simp_tac(srw_ss())[opcode_def]
+    \\ blastLib.BBLAST_TAC
+  )
+  THENL
+
+
+  \\ TRY(rename1 ‘opcode opc‘ \\ Cases_on ‘opc’ \\ qhdtm_x_assum ‘opcode‘ mp_tac \\ simp_tac(srw_ss())[opcode_def])
+  \\ ntac 2 (pop_assum mp_tac)
+  \\ rpt (pop_assum kall_tac)
+  \\ TRY(rename1`opcode opc` \\ Cases_on`opc` \\ fs[opcode_def])
+  \\ rpt (pop_assum mp_tac)
+   \\ blastLib.BBLAST_TAC
+End
+
+open cv_transLib cv_stdTheory;
 
 Definition parse_opcode_exec_def:
   parse_opcode_exec (opc:byte list)
@@ -264,7 +550,7 @@ End
 
 val _ = cv_trans parse_opcode_exec_def;
 
-        
+
         open Tactic;
 
 Triviality parse_opcode_eqv_parse_opcode_exec:
@@ -294,183 +580,6 @@ QED
 
 val _ = cv_auto_trans parse_opcode_def;
 (* TODO: parse_opcode_unique theorem *)
-
-Definition static_gas_def[simp]:
-    static_gas Stop           = 0
-  ∧ static_gas Add            = 3
-  ∧ static_gas Mul            = 5
-  ∧ static_gas Sub            = 3
-  ∧ static_gas Div            = 5
-  ∧ static_gas SDiv           = 5
-  ∧ static_gas Mod            = 5
-  ∧ static_gas SMod           = 5
-  ∧ static_gas AddMod         = 8
-  ∧ static_gas MulMod         = 8
-  ∧ static_gas Exp            = 10
-  ∧ static_gas SignExtend     = 5
-  ∧ static_gas LT             = 3
-  ∧ static_gas GT             = 3
-  ∧ static_gas SLT            = 3
-  ∧ static_gas SGT            = 3
-  ∧ static_gas Eq             = 3
-  ∧ static_gas IsZero         = 3
-  ∧ static_gas And            = 3
-  ∧ static_gas Or             = 3
-  ∧ static_gas XOr            = 3
-  ∧ static_gas Not            = 3
-  ∧ static_gas Byte           = 3
-  ∧ static_gas ShL            = 3
-  ∧ static_gas ShR            = 3
-  ∧ static_gas SAR            = 3
-  ∧ static_gas Keccak256      = 30
-  ∧ static_gas Address        = 30
-  ∧ static_gas Balance        = 0
-  ∧ static_gas Origin         = 2
-  ∧ static_gas Caller         = 2
-  ∧ static_gas CallValue      = 2
-  ∧ static_gas CallDataLoad   = 3
-  ∧ static_gas CallDataSize   = 2
-  ∧ static_gas CallDataCopy   = 3
-  ∧ static_gas CodeSize       = 2
-  ∧ static_gas CodeCopy       = 3
-  ∧ static_gas GasPrice       = 2
-  ∧ static_gas ExtCodeSize    = 0
-  ∧ static_gas ExtCodeCopy    = 0
-  ∧ static_gas ReturnDataSize = 2
-  ∧ static_gas ReturnDataCopy = 3
-  ∧ static_gas ExtCodeHash    = 0
-  ∧ static_gas BlockHash      = 20
-  ∧ static_gas CoinBase       = 2
-  ∧ static_gas TimeStamp      = 2
-  ∧ static_gas Number         = 2
-  ∧ static_gas PrevRandao     = 2
-  ∧ static_gas GasLimit       = 2
-  ∧ static_gas ChainId        = 2
-  ∧ static_gas SelfBalance    = 5
-  ∧ static_gas BaseFee        = 2
-  ∧ static_gas Pop            = 2
-  ∧ static_gas MLoad          = 3
-  ∧ static_gas MStore         = 3
-  ∧ static_gas MStore8        = 3
-  ∧ static_gas SLoad          = 0
-  ∧ static_gas SStore         = 0
-  ∧ static_gas Jump           = 8
-  ∧ static_gas JumpI          = 10
-  ∧ static_gas PC             = 2
-  ∧ static_gas MSize          = 2
-  ∧ static_gas Gas            = 2
-  ∧ static_gas JumpDest       = 1
-  ∧ static_gas (Push n w)     = (if n = 0w then 2 else 3)
-  ∧ static_gas (Dup n)        = 3
-  ∧ static_gas (Swap n)       = 3
-  ∧ static_gas (Log n)        = 375
-  ∧ static_gas Create         = 32000
-  ∧ static_gas Call           = 0
-  ∧ static_gas CallCode       = 0
-  ∧ static_gas Return         = 0
-  ∧ static_gas DelegateCall   = 0
-  ∧ static_gas Create2        = 32000
-  ∧ static_gas StaticCall     = 0
-  ∧ static_gas Revert         = 0
-End
-
-
-* finish if necessary
-Theorem parse_opcode_cond_thm:
-  parse_opcode (opc::data: byte list) =
-  if opc = n2w 0x00 then SOME Stop else
-  if opc = n2w 0x01 then SOME Add else
-  if opc = n2w 0x02 then SOME Mul else
-  if opc = n2w 0x03 then SOME Sub else
-  if opc = n2w 0x04 then SOME Div else
-  if opc = n2w 0x05 then SOME SDiv else
-  if opc = n2w 0x06 then SOME Mod else
-  if opc = n2w 0x07 then SOME SMod else
-  if opc = n2w 0x08 then SOME AddMod else
-  if opc = n2w 0x09 then SOME MulMod else
-  if opc = n2w 0x0a then SOME Exp else
-  if opc = n2w 0x0b then SOME SignExtend else
-  if opc = n2w 0x10 then SOME LT else
-  if opc = n2w 0x11 then SOME GT else
-  if opc = n2w 0x12 then SOME SLT else
-  if opc = n2w 0x13 then SOME SGT else
-  if opc = n2w 0x14 then SOME Eq else
-  if opc = n2w 0x15 then SOME IsZero else
-  if opc = n2w 0x16 then SOME And else
-  if opc = n2w 0x17 then SOME Or else
-  if opc = n2w 0x18 then SOME XOr else
-  if opc = n2w 0x19 then SOME Not else
-  if opc = n2w 0x1a then SOME Byte else
-  if opc = n2w 0x1b then SOME ShL else
-  if opc = n2w 0x1c then SOME ShR else
-  if opc = n2w 0x1d then SOME SAR else
-  if opc = n2w 0x20 then SOME Keccak256 else
-  if opc = n2w 0x30 then SOME Address else
-  if opc = n2w 0x31 then SOME Balance else
-  if opc = n2w 0x32 then SOME Origin else
-  if opc = n2w 0x33 then SOME Caller else
-  if opc = n2w 0x34 then SOME CallValue else
-  if opc = n2w 0x35 then SOME CallDataLoad else
-  if opc = n2w 0x36 then SOME CallDataSize else
-  if opc = n2w 0x37 then SOME CallDataCopy else
-  if opc = n2w 0x38 then SOME CodeSize else
-  if opc = n2w 0x39 then SOME CodeCopy else
-  if opc = n2w 0x3a then SOME GasPrice else
-  if opc = n2w 0x3b then SOME ExtCodeSize else
-  if opc = n2w 0x3c then SOME ExtCodeCopy else
-  if opc = n2w 0x3d then SOME ReturnDataSize else
-  if opc = n2w 0x3e then SOME ReturnDataCopy else
-  if opc = n2w 0x3f then SOME ExtCodeHash else
-  if opc = n2w 0x40 then SOME BlockHash else
-  if opc = n2w 0x41 then SOME CoinBase else
-  if opc = n2w 0x42 then SOME TimeStamp else
-  if opc = n2w 0x43 then SOME Number else
-  if opc = n2w 0x44 then SOME PrevRandao else
-  if opc = n2w 0x45 then SOME GasLimit else
-  if opc = n2w 0x46 then SOME ChainId else
-  if opc = n2w 0x47 then SOME SelfBalance else
-  if opc = n2w 0x48 then SOME BaseFee else
-  if opc = n2w 0x50 then SOME Pop else
-  if opc = n2w 0x51 then SOME MLoad else
-  if opc = n2w 0x52 then SOME MStore else
-  if opc = n2w 0x53 then SOME MStore8 else
-  if opc = n2w 0x54 then SOME SLoad else
-  if opc = n2w 0x55 then SOME SStore else
-  if opc = n2w 0x56 then SOME Jump else
-  if opc = n2w 0x57 then SOME JumpI else
-  if opc = n2w 0x58 then SOME PC else
-  if opc = n2w 0x59 then SOME MSize else
-  if opc = n2w 0x5a then SOME Gas else
-  if opc = n2w 0x5b then SOME JumpDest else
-  if opc = n2w 0x5f then SOME (Push 0w data) else
-
-≤ opc ∧ opc ≤ n2w 0x7f then SOME (Push (w2w opc - n2w 0x5f) data) else
-  if n2w 0x80 ≤ opc ∧ opc ≤ n2w 0x8f then SOME (Dup (w2w opc - n2w 0x81)) else
-  if n2w 0x90 ≤ opc ∧ opc ≤ n2w 0x9f then SOME (Swap (w2w opc - n2w 0x91)) else
-  if n2w 0xa0 ≤ opc ∧ opc ≤ n2w 0xa4 then SOME (Log (w2w opc - n2w 0xa0)) else
-  if opc = n2w 0xf0 then SOME Create else
-  if opc = n2w 0xf1 then SOME Call else
-  if opc = n2w 0xf2 then SOME CallCode else
-  if opc = n2w 0xf3 then SOME Return else
-  if opc = n2w 0xf4 then SOME DelegateCall else
-  if opc = n2w 0xf5 then SOME Create2 else
-  if opc = n2w 0xfa then SOME StaticCall else
-  if opc = n2w 0xfd then SOME Revert else
-  NONE
-Proof
-  simp[parse_opcode_def]
-  \\ DEEP_INTRO_TAC some_intro
-  \\ rw[]
-  \\ TRY(rename1`opcode opc` \\ Cases_on`opc` \\  qpat_x_assum`_ _ _`mp_tac \\ simp_tac(srw_ss())[opcode_def] \\ blastLib.BBLAST_TAC)
-
-  
-  \\ TRY(rename1 ‘opcode opc‘ \\ Cases_on ‘opc’ \\ qhdtm_x_assum ‘opcode‘ mp_tac \\ simp_tac(srw_ss())[opcode_def])
-  \\ ntac 2 (pop_assum mp_tac)
-  \\ rpt (pop_assum kall_tac)       
-  \\ TRY(rename1`opcode opc` \\ Cases_on`opc` \\ fs[opcode_def])
-  \\ rpt (pop_assum mp_tac)
-   \\ blastLib.BBLAST_TAC
-End
-
+*)
 
 val _ = export_theory();
